theories/Feature.v
@@ -1,0 +1,710 @@
+From Stdlib Require Import MSets.
+From PackageCalculus Require Import Prelude Core.
+
+Create HintDb cmp_feat.
+Create Rewrite HintDb cmp_feat.
+
+Module Feature (N V F : UsualOrderedType).
+  Module C := Core N V.
+  Module Pkg := C.Pkg.
+  Module PkgSet := C.PkgSet.
+  Module VSet := C.VSet.
+
+  Module FSet := FSetUOT F.
+
+  Module Featured := PairUOT Pkg FSet.AsUOT.
+  Module FeaturedSet := FSetUOT Featured.
+
+  Module PkgF := PairUOT Pkg F.
+  Module SupportSet := FSetUOT PkgF.
+
+  Module VSFS := PairUOT VSet.AsUOT FSet.AsUOT.
+  Module Dependees := PairUOT N VSFS.
+  Module FeatDepElt := PairUOT Pkg Dependees.
+  Module FeatDepRel := FSetUOT FeatDepElt.
+
+  Module AddlDepElt := PairUOT PkgF Dependees.
+  Module AddlDepRel := FSetUOT AddlDepElt.
+
+  Record IsResolution
+      (R : PkgSet.t) (support : SupportSet.t)
+      (Df : FeatDepRel.t) (Da : AddlDepRel.t)
+      (r : Pkg.t) (S : FeaturedSet.t) : Prop :=
+    { res_no_root_support : forall f, ~ SupportSet.In (r, f) support
+    ; res_subset : forall p fs, FeaturedSet.In (p, fs) S -> PkgSet.In p R
+    ; res_root_mem : FeaturedSet.In (r, FSet.empty) S
+    ; res_dep_closure :
+        forall p fs_p, FeaturedSet.In (p, fs_p) S ->
+        forall n vs fs, FeatDepRel.In (p, (n, (vs, fs))) Df ->
+        exists v, VSet.In v vs /\
+          exists fs', FSet.Subset fs fs' /\ FeaturedSet.In ((n, v), fs') S
+    ; res_addl_dep_closure :
+        forall p fs_p, FeaturedSet.In (p, fs_p) S ->
+        forall f, FSet.In f fs_p ->
+        forall n vs fs, AddlDepRel.In ((p, f), (n, (vs, fs))) Da ->
+        exists v, VSet.In v vs /\
+          exists fs', FSet.Subset fs fs' /\ FeaturedSet.In ((n, v), fs') S
+    ; res_feature_unification :
+        forall n v v' fs fs',
+          FeaturedSet.In ((n, v), fs) S ->
+          FeaturedSet.In ((n, v'), fs') S -> fs = fs'
+    ; res_version_unique :
+        forall n v v' fs fs',
+          FeaturedSet.In ((n, v), fs) S ->
+          FeaturedSet.In ((n, v'), fs') S -> v = v'
+    ; res_support_mem :
+        forall n v fs f,
+          FeaturedSet.In ((n, v), fs) S -> FSet.In f fs ->
+          SupportSet.In ((n, v), f) support }.
+
+  Module Reduction.
+    Module NFPair := PairUOT N F.
+    Module NFF := UOTCompareFacts NFPair.
+    Module NF := UOTCompareFacts N.
+    #[local] Hint Rewrite NFF.compare_eq_iff NF.compare_eq_iff : cmp_feat.
+    #[local] Hint Extern 1 => cmp_by NFF.compare_antisym : cmp_feat.
+    #[local] Hint Extern 1 => cmp_by NF.compare_antisym : cmp_feat.
+    #[local] Hint Extern 1 => cmp_by NFF.compare_lt_trans : cmp_feat.
+    #[local] Hint Extern 1 => cmp_by NF.compare_lt_trans : cmp_feat.
+
+    Module Name.
+      Inductive name : Type :=
+      | Orig (n : N.t)
+      | FeatPkg (n : N.t) (f : F.t).
+      Definition t := name.
+
+      Definition compare (x y : t) : comparison :=
+        match x, y with
+        | Orig n1, Orig n2 => N.compare n1 n2
+        | Orig _, FeatPkg _ _ => Lt
+        | FeatPkg _ _, Orig _ => Gt
+        | FeatPkg n1 f1, FeatPkg n2 f2 => NFPair.compare (n1, f1) (n2, f2)
+        end.
+
+      Lemma compare_eq_iff : forall x y, compare x y = Eq <-> x = y.
+      Proof. cmp_eq_iff cmp_feat. Qed.
+
+      Lemma compare_antisym : forall x y, compare y x = CompOpp (compare x y).
+      Proof. cmp_antisym cmp_feat. Qed.
+
+      Lemma compare_lt_trans : forall x y z,
+          compare x y = Lt -> compare y z = Lt -> compare x z = Lt.
+      Proof. cmp_lt_trans cmp_feat. Qed.
+    End Name.
+    Module NameOT := UOTFromCompare Name.
+
+    Module T := Core NameOT V.
+
+    (* The target core is a distinct instantiation even though versions are
+       unchanged, so version sets are rebuilt element-wise. *)
+    Module SOvt := SetOps V V VSet T.VSet.
+    Definition embedVS (vs : VSet.t) : T.VSet.t :=
+      SOvt.map (fun v => v) vs.
+
+    Definition embedPkg (p : Pkg.t) : T.Pkg.t :=
+      let '(n, v) := p in (Name.Orig n, v).
+
+    Module SOpt := SetOps Pkg T.Pkg PkgSet T.PkgSet.
+    Definition embedSet (S : PkgSet.t) : T.PkgSet.t :=
+      SOpt.map embedPkg S.
+
+    Module SOst := SetOps PkgF T.Pkg SupportSet T.PkgSet.
+    Definition featPkgReal (R : PkgSet.t)
+        (support : SupportSet.t) : T.PkgSet.t :=
+      SOst.filterMap (fun '((n, v), f) =>
+          if PkgSet.mem (n, v) R
+          then Some (Name.FeatPkg n f, v)
+          else None)
+        support.
+
+    Definition reduceReal (R : PkgSet.t) (support : SupportSet.t)
+        : T.PkgSet.t :=
+      T.PkgSet.union (embedSet R) (featPkgReal R support).
+
+    Module SOsd := SetOps PkgF T.DepElt SupportSet T.DepRel.
+    Definition supportEdges (R : PkgSet.t)
+        (support : SupportSet.t) : T.DepRel.t :=
+      SOsd.filterMap (fun '((n, v), f) =>
+          if PkgSet.mem (n, v) R
+          then Some ((Name.FeatPkg n f, v),
+                     (Name.Orig n, T.VSet.singleton v))
+          else None)
+        support.
+
+    Module SOfd := SetOps FeatDepElt T.DepElt FeatDepRel T.DepRel.
+    Definition featDepOrigEdges (Df : FeatDepRel.t) : T.DepRel.t :=
+      SOfd.filterMap (fun '(p, (n, (vs, fs))) =>
+          if FSet.is_empty fs
+          then Some (embedPkg p, (Name.Orig n, embedVS vs))
+          else None)
+        Df.
+
+    Module SOfsd := SetOps F T.DepElt FSet T.DepRel.
+    Definition featDepFeatPkgEdges (Df : FeatDepRel.t) : T.DepRel.t :=
+      SOfd.unionMap (fun '(p, (n, (vs, fs))) =>
+          if FSet.is_empty fs then T.DepRel.empty
+          else SOfsd.map (fun f =>
+                   (embedPkg p, (Name.FeatPkg n f, embedVS vs)))
+                 fs)
+        Df.
+
+    Module SOad := SetOps AddlDepElt T.DepElt AddlDepRel T.DepRel.
+    Definition addlDepOrigEdges (Da : AddlDepRel.t) : T.DepRel.t :=
+      SOad.filterMap (fun '(((n, v), f), (m, (vs, fs))) =>
+          if FSet.is_empty fs
+          then Some ((Name.FeatPkg n f, v), (Name.Orig m, embedVS vs))
+          else None)
+        Da.
+
+    Definition addlDepFeatPkgEdges (Da : AddlDepRel.t) : T.DepRel.t :=
+      SOad.unionMap (fun '(((n, v), f), (m, (vs, fs))) =>
+          if FSet.is_empty fs then T.DepRel.empty
+          else SOfsd.map (fun f' =>
+                   ((Name.FeatPkg n f, v),
+                    (Name.FeatPkg m f', embedVS vs)))
+                 fs)
+        Da.
+
+    Definition reduceDeps (R : PkgSet.t) (support : SupportSet.t)
+        (Df : FeatDepRel.t) (Da : AddlDepRel.t) : T.DepRel.t :=
+      T.DepRel.union (supportEdges R support)
+        (T.DepRel.union (featDepOrigEdges Df)
+           (T.DepRel.union (featDepFeatPkgEdges Df)
+              (T.DepRel.union (addlDepOrigEdges Da)
+                 (addlDepFeatPkgEdges Da)))).
+
+    Lemma mem_embedVS : forall vs v, T.VSet.In v (embedVS vs) <-> VSet.In v vs.
+    Proof.
+      intros vs v; unfold embedVS.
+      exact (SOvt.mem_map_inj (fun w => w) vs v (fun x y H => H)).
+    Qed.
+
+    Lemma mem_featPkgReal : forall R support q,
+        T.PkgSet.In q (featPkgReal R support) <->
+        exists n v f, SupportSet.In ((n, v), f) support /\ PkgSet.In (n, v) R /\
+          q = (Name.FeatPkg n f, v).
+    Proof.
+      intros R support q; unfold featPkgReal; rewrite SOst.mem_filterMap.
+      split.
+      - intros [[[pn pv] f0] [Hs Hq]]; cbn beta iota in Hq.
+        destruct (PkgSet.mem (pn, pv) R) eqn:Em; [| discriminate].
+        injection Hq as <-.
+        exists pn, pv, f0; repeat split;
+          [exact Hs | apply PkgSet.mem_spec; exact Em].
+      - intros [n [v [f0 [Hs [HR ->]]]]].
+        exists ((n, v), f0); split; [exact Hs | cbn beta iota].
+        rewrite <- PkgSet.mem_spec in HR; rewrite HR; reflexivity.
+    Qed.
+
+    Lemma mem_reduceReal : forall R support q,
+        T.PkgSet.In q (reduceReal R support) <->
+        (exists p, PkgSet.In p R /\ q = embedPkg p) \/
+        (exists n v f, SupportSet.In ((n, v), f) support /\
+           PkgSet.In (n, v) R /\
+           q = (Name.FeatPkg n f, v)).
+    Proof.
+      intros R support q; unfold reduceReal, embedSet.
+      rewrite T.PkgSet.union_spec, SOpt.mem_map, mem_featPkgReal; reflexivity.
+    Qed.
+
+    Lemma mem_supportEdges :
+      forall R support (q : T.Pkg.t) (m : NameOT.t) (ws : T.VSet.t),
+        T.DepRel.In (q, (m, ws)) (supportEdges R support) <->
+        exists n v f, SupportSet.In ((n, v), f) support /\ PkgSet.In (n, v) R /\
+          q = (Name.FeatPkg n f, v) /\ m = Name.Orig n /\
+          ws = T.VSet.singleton v.
+    Proof.
+      intros R support q m ws; unfold supportEdges; rewrite SOsd.mem_filterMap.
+      split.
+      - intros [[[pn pv] f0] [Hs Hy]]; cbn beta iota in Hy.
+        destruct (PkgSet.mem (pn, pv) R) eqn:Em; [| discriminate].
+        injection Hy as <- <- <-.
+        exists pn, pv, f0; repeat split;
+          [exact Hs | apply PkgSet.mem_spec; exact Em].
+      - intros [n [v [f0 [Hs [HR [Hsrc [Htn Htvs]]]]]]]; subst q m ws.
+        exists ((n, v), f0); split; [exact Hs | cbn beta iota].
+        rewrite <- PkgSet.mem_spec in HR; rewrite HR; reflexivity.
+    Qed.
+
+    Lemma mem_featDepOrigEdges :
+      forall Df (q : T.Pkg.t) (m : NameOT.t) (ws : T.VSet.t),
+        T.DepRel.In (q, (m, ws)) (featDepOrigEdges Df) <->
+        exists p n vs, FeatDepRel.In (p, (n, (vs, FSet.empty))) Df /\
+          q = embedPkg p /\ m = Name.Orig n /\ ws = embedVS vs.
+    Proof.
+      intros Df q m ws; unfold featDepOrigEdges; rewrite SOfd.mem_filterMap.
+      split.
+      - intros [[p [m0 [vs0 fs0]]] [He2 Hy]]; cbn beta iota in Hy.
+        destruct (FSet.is_empty fs0) eqn:E0; [| discriminate].
+        injection Hy as <- <- <-.
+        apply FSet.is_empty_iff in E0; subst fs0.
+        exists p, m0, vs0; repeat split; exact He2.
+      - intros [p [m0 [vs0 [He2 [Hsrc [Htn Htvs]]]]]]; subst q m ws.
+        exists (p, (m0, (vs0, FSet.empty))); split; [exact He2 | simpl];
+          reflexivity.
+    Qed.
+
+    Lemma mem_featDepFeatPkgEdges :
+      forall Df (q : T.Pkg.t) (m : NameOT.t) (ws : T.VSet.t),
+        T.DepRel.In (q, (m, ws)) (featDepFeatPkgEdges Df) <->
+        exists p n vs fs f, FeatDepRel.In (p, (n, (vs, fs))) Df /\
+          FSet.is_empty fs = false /\ FSet.In f fs /\
+          q = embedPkg p /\ m = Name.FeatPkg n f /\ ws = embedVS vs.
+    Proof.
+      intros Df q m ws; unfold featDepFeatPkgEdges; rewrite SOfd.mem_unionMap.
+      split.
+      - intros [[p [m0 [vs0 fs0]]] [He3 Hy]]; cbn beta iota in Hy.
+        destruct (FSet.is_empty fs0) eqn:E0; [destruct (SOfd.empty_in _ Hy) |].
+        apply SOfsd.mem_map in Hy; destruct Hy as [f [Hf Hy]].
+        injection Hy as -> -> ->.
+        exists p, m0, vs0, fs0, f; repeat split; assumption.
+      - intros [p [m0 [vs0 [fs0 [f [He3 [E0 [Hf [Hsrc [Htn Htvs]]]]]]]]]];
+          subst q m ws.
+        exists (p, (m0, (vs0, fs0))); split; [exact He3 | cbn beta iota].
+        rewrite E0.
+        apply SOfsd.mem_map; exists f; split; [exact Hf | reflexivity].
+    Qed.
+
+    Lemma mem_addlDepOrigEdges :
+      forall Da (q : T.Pkg.t) (m : NameOT.t) (ws : T.VSet.t),
+        T.DepRel.In (q, (m, ws)) (addlDepOrigEdges Da) <->
+        exists n v f m' vs,
+          AddlDepRel.In (((n, v), f), (m', (vs, FSet.empty))) Da /\
+          q = (Name.FeatPkg n f, v) /\ m = Name.Orig m' /\ ws = embedVS vs.
+    Proof.
+      intros Da q m ws; unfold addlDepOrigEdges; rewrite SOad.mem_filterMap.
+      split.
+      - intros [[[[pn pv] f0] [m0 [vs0 fs0]]] [He4 Hy]]; cbn beta iota in Hy.
+        destruct (FSet.is_empty fs0) eqn:E0; [| discriminate].
+        injection Hy as <- <- <-.
+        apply FSet.is_empty_iff in E0; subst fs0.
+        exists pn, pv, f0, m0, vs0; repeat split; exact He4.
+      - intros [n [v [f0 [m0 [vs0 [He4 [Hsrc [Htn Htvs]]]]]]]]; subst q m ws.
+        exists (((n, v), f0), (m0, (vs0, FSet.empty)));
+          split; [exact He4 | simpl]; reflexivity.
+    Qed.
+
+    Lemma mem_addlDepFeatPkgEdges :
+      forall Da (q : T.Pkg.t) (m : NameOT.t) (ws : T.VSet.t),
+        T.DepRel.In (q, (m, ws)) (addlDepFeatPkgEdges Da) <->
+        exists n v f m' vs fs f',
+          AddlDepRel.In (((n, v), f), (m', (vs, fs))) Da /\
+          FSet.is_empty fs = false /\ FSet.In f' fs /\
+          q = (Name.FeatPkg n f, v) /\ m = Name.FeatPkg m' f' /\
+          ws = embedVS vs.
+    Proof.
+      intros Da q m ws; unfold addlDepFeatPkgEdges; rewrite SOad.mem_unionMap.
+      split.
+      - intros [[[[pn pv] f0] [m0 [vs0 fs0]]] [He5 Hy]]; cbn beta iota in Hy.
+        destruct (FSet.is_empty fs0) eqn:E0; [destruct (SOad.empty_in _ Hy) |].
+        apply SOfsd.mem_map in Hy; destruct Hy as [f' [Hf' Hy]].
+        injection Hy as -> -> ->.
+        exists pn, pv, f0, m0, vs0, fs0, f'; repeat split; assumption.
+      - intros [n [v [f0 [m0 [vs0 [fs0 [f'
+                  [He5 [E0 [Hf' [Hsrc [Htn Htvs]]]]]]]]]]]]; subst q m ws.
+        exists (((n, v), f0), (m0, (vs0, fs0)));
+          split; [exact He5 | cbn beta iota].
+        rewrite E0.
+        apply SOfsd.mem_map; exists f'; split; [exact Hf' | reflexivity].
+    Qed.
+
+    Lemma mem_reduceDeps :
+      forall R support Df Da (q : T.Pkg.t) (m : NameOT.t) (ws : T.VSet.t),
+        T.DepRel.In (q, (m, ws)) (reduceDeps R support Df Da) <->
+        (exists n v f, SupportSet.In ((n, v), f) support /\
+           PkgSet.In (n, v) R /\
+           q = (Name.FeatPkg n f, v) /\ m = Name.Orig n /\
+           ws = T.VSet.singleton v) \/
+        (exists p n vs, FeatDepRel.In (p, (n, (vs, FSet.empty))) Df /\
+           q = embedPkg p /\ m = Name.Orig n /\ ws = embedVS vs) \/
+        (exists p n vs fs f, FeatDepRel.In (p, (n, (vs, fs))) Df /\
+           FSet.is_empty fs = false /\ FSet.In f fs /\
+           q = embedPkg p /\ m = Name.FeatPkg n f /\ ws = embedVS vs) \/
+        (exists n v f m' vs,
+           AddlDepRel.In (((n, v), f), (m', (vs, FSet.empty))) Da /\
+           q = (Name.FeatPkg n f, v) /\ m = Name.Orig m' /\ ws = embedVS vs) \/
+        (exists n v f m' vs fs f',
+           AddlDepRel.In (((n, v), f), (m', (vs, fs))) Da /\
+           FSet.is_empty fs = false /\ FSet.In f' fs /\
+           q = (Name.FeatPkg n f, v) /\ m = Name.FeatPkg m' f' /\
+           ws = embedVS vs).
+    Proof.
+      intros R support Df Da q m ws; unfold reduceDeps.
+      rewrite !T.DepRel.union_spec, mem_supportEdges, mem_featDepOrigEdges,
+        mem_featDepFeatPkgEdges, mem_addlDepOrigEdges,
+        mem_addlDepFeatPkgEdges.
+      tauto.
+    Qed.
+
+    Module SOtf := SetOps T.Pkg F T.PkgSet FSet.
+    (* Decoding reads the features off the resolution rather than sieving the
+       feature universe by membership in it: the two agree, but only this
+       direction is defined when F is unbounded, as a package ecosystem's
+       feature names are. *)
+    Definition featsOf (n : N.t) (v : V.t) (S : T.PkgSet.t) : FSet.t :=
+      SOtf.filterMap (fun q =>
+          match q with
+          | (Name.FeatPkg n' f, v') =>
+              if T.Pkg.eq_dec (Name.FeatPkg n' f, v') (Name.FeatPkg n f, v)
+              then Some f
+              else None
+          | _ => None
+          end)
+        S.
+
+    Lemma featsOf_spec : forall n v S f,
+        FSet.In f (featsOf n v S) <-> T.PkgSet.In (Name.FeatPkg n f, v) S.
+    Proof.
+      intros n v S f; unfold featsOf; rewrite SOtf.mem_filterMap.
+      split.
+      - intros [[[n' | n' f'] v'] [HS He]]; cbn beta iota in He;
+          [discriminate |].
+        destruct (T.Pkg.eq_dec (Name.FeatPkg n' f', v') (Name.FeatPkg n f', v))
+          as [E | NE]; [| discriminate].
+        injection He as <-; rewrite <- E; exact HS.
+      - intro HS; exists (Name.FeatPkg n f, v);
+          split; [exact HS | cbn beta iota].
+        destruct (T.Pkg.eq_dec (Name.FeatPkg n f, v) (Name.FeatPkg n f, v))
+          as [_ | NE]; [reflexivity | exfalso; exact (NE eq_refl)].
+    Qed.
+
+    Module SOts := SetOps T.Pkg Featured T.PkgSet FeaturedSet.
+    Definition featureResolution (S : T.PkgSet.t) : FeaturedSet.t :=
+      SOts.filterMap (fun p' =>
+          match p' with
+          | (Name.Orig n, v) => Some ((n, v), featsOf n v S)
+          | _ => None
+          end)
+        S.
+
+    Lemma mem_featureResolution : forall (S : T.PkgSet.t) (y : Featured.t),
+        FeaturedSet.In y (featureResolution S) <->
+        exists n v,
+          T.PkgSet.In (Name.Orig n, v) S /\ y = ((n, v), featsOf n v S).
+    Proof.
+      intros S y; unfold featureResolution; rewrite SOts.mem_filterMap.
+      split.
+      - intros [[[n | n f] v] [HeS Hy]]; cbn beta iota in Hy; [| discriminate].
+        injection Hy as <-; exists n, v; split; [exact HeS | reflexivity].
+      - intros [n [v [HS ->]]].
+        exists (Name.Orig n, v); split; [exact HS | reflexivity].
+    Qed.
+
+    Theorem feature_soundness :
+      forall (R : PkgSet.t) (support : SupportSet.t)
+             (Df : FeatDepRel.t) (Da : AddlDepRel.t)
+             (r : Pkg.t) (S : T.PkgSet.t),
+        T.IsResolution (reduceReal R support) (reduceDeps R support Df Da)
+          (embedPkg r) S ->
+        (forall f, ~ SupportSet.In (r, f) support) ->
+        IsResolution R support Df Da r (featureResolution S).
+    Proof.
+      intros R support Df Da r S Hres Hnosupp.
+      destruct Hres as [Hsub Hroot Hdep Huniq].
+      destruct r as [rn rv].
+      unfold embedPkg in Hroot; simpl in Hroot.
+      assert (HorigR : forall n v,
+                 T.PkgSet.In (Name.Orig n, v) S -> PkgSet.In (n, v) R).
+      { intros n v HS.
+        pose proof (Hsub _ HS) as HF; rewrite mem_reduceReal in HF.
+        destruct HF as [[p [HpR Hq]] | [n' [v' [f' [Hsupp [HR Hq]]]]]].
+        - destruct p as [pn pv]; unfold embedPkg in Hq; simpl in Hq.
+          injection Hq as E1 E2; subst pn pv; exact HpR.
+        - discriminate Hq. }
+      assert (HnorootF : forall f, ~ T.PkgSet.In (Name.FeatPkg rn f, rv) S).
+      { intros f HS.
+        pose proof (Hsub _ HS) as HF; rewrite mem_reduceReal in HF.
+        destruct HF as [[p [HpR Hq]] | [n' [v' [f' [Hsupp [HR Hq]]]]]].
+        - destruct p as [pn pv]; unfold embedPkg in Hq; simpl in Hq;
+            discriminate Hq.
+        - injection Hq as E1 E2 E3; subst n' f' v'.
+          exact (Hnosupp _ Hsupp). }
+      assert (HfeatOrig : forall n f v,
+                 T.PkgSet.In (Name.FeatPkg n f, v) S ->
+                 T.PkgSet.In (Name.Orig n, v) S).
+      { intros n f v HS.
+        pose proof (Hsub _ HS) as HF; rewrite mem_reduceReal in HF.
+        destruct HF as [[p [HpR Hq]] | [n' [v' [f' [Hsupp [HR Hq]]]]]].
+        - destruct p as [pn pv]; unfold embedPkg in Hq; simpl in Hq;
+            discriminate Hq.
+        - injection Hq as E1 E2 E3; subst n' f' v'.
+          assert (Hd : T.DepRel.In
+                         ((Name.FeatPkg n f, v),
+                          (Name.Orig n, T.VSet.singleton v))
+                         (reduceDeps R support Df Da)).
+          { rewrite mem_reduceDeps.
+            left; exists n, v, f.
+            split; [exact Hsupp | split; [exact HR |]].
+            split; [reflexivity | split; reflexivity]. }
+          destruct (Hdep _ HS _ _ Hd) as [v0 [Hv0 Hv0S]].
+          rewrite SOvt.singleton_in in Hv0; subst v0.
+          exact Hv0S. }
+      constructor.
+      - exact Hnosupp.
+      - intros p fs Hmem.
+        apply mem_featureResolution in Hmem;
+          destruct Hmem as [n [v [HS Heq]]].
+        injection Heq as E1 E2; subst p.
+        exact (HorigR n v HS).
+      - assert (Hfe : featsOf rn rv S = FSet.empty).
+        { apply FSet.ext; intro f; rewrite featsOf_spec; split; intro H.
+          + exfalso; exact (HnorootF f H).
+          + exfalso; exact (FSet.empty_spec H). }
+        rewrite <- Hfe.
+        apply mem_featureResolution; exists rn, rv;
+          split; [exact Hroot | reflexivity].
+      - intros p fs_p Hmem n vs fs Hdf.
+        apply mem_featureResolution in Hmem;
+          destruct Hmem as [pn [pv [HpS Heq]]].
+        injection Heq as E1 E2; subst p fs_p.
+        destruct (FSet.is_empty fs) eqn:E.
+        + apply FSet.is_empty_iff in E; subst fs.
+          assert (Hd : T.DepRel.In
+                         ((Name.Orig pn, pv), (Name.Orig n, embedVS vs))
+                         (reduceDeps R support Df Da)).
+          { rewrite mem_reduceDeps.
+            right; left; exists (pn, pv), n, vs.
+            split; [exact Hdf | split; [reflexivity | split; reflexivity]]. }
+          destruct (Hdep _ HpS _ _ Hd) as [v [Hv HvS]].
+          rewrite mem_embedVS in Hv.
+          exists v; split; [exact Hv |].
+          exists (featsOf n v S); split.
+          * intros x Hx; exfalso; exact (FSet.empty_spec Hx).
+          * apply mem_featureResolution; exists n, v;
+              split; [exact HvS | reflexivity].
+        + destruct (FSet.choose_nonempty _ E) as [f0 Hf0].
+          assert (Hd0 : T.DepRel.In
+                          ((Name.Orig pn, pv), (Name.FeatPkg n f0, embedVS vs))
+                          (reduceDeps R support Df Da)).
+          { rewrite mem_reduceDeps.
+            right; right; left; exists (pn, pv), n, vs, fs, f0.
+            split; [exact Hdf | split; [exact E | split; [exact Hf0 |]]].
+            split; [reflexivity | split; reflexivity]. }
+          destruct (Hdep _ HpS _ _ Hd0) as [v [Hv HvS]].
+          rewrite mem_embedVS in Hv.
+          pose proof (HfeatOrig _ _ _ HvS) as HvO.
+          exists v; split; [exact Hv |].
+          exists (featsOf n v S); split.
+          * intros f' Hf'; rewrite featsOf_spec.
+            assert (Hd' : T.DepRel.In
+                            ((Name.Orig pn, pv),
+                             (Name.FeatPkg n f', embedVS vs))
+                            (reduceDeps R support Df Da)).
+            { rewrite mem_reduceDeps.
+              right; right; left; exists (pn, pv), n, vs, fs, f'.
+              split; [exact Hdf | split; [exact E | split; [exact Hf' |]]].
+              split; [reflexivity | split; reflexivity]. }
+            destruct (Hdep _ HpS _ _ Hd') as [v' [Hv' Hv'S]].
+            pose proof (HfeatOrig _ _ _ Hv'S) as Hv'O.
+            assert (Ev : v = v') by exact (Huniq (Name.Orig n) v v' HvO Hv'O).
+            rewrite Ev; exact Hv'S.
+          * apply mem_featureResolution; exists n, v;
+              split; [exact HvO | reflexivity].
+      - intros p fs_p Hmem f Hf n vs fs Hda.
+        apply mem_featureResolution in Hmem;
+          destruct Hmem as [pn [pv [HpS Heq]]].
+        injection Heq as E1 E2; subst p fs_p.
+        rewrite featsOf_spec in Hf.
+        destruct (FSet.is_empty fs) eqn:E.
+        + apply FSet.is_empty_iff in E; subst fs.
+          assert (Hd : T.DepRel.In
+                         ((Name.FeatPkg pn f, pv), (Name.Orig n, embedVS vs))
+                         (reduceDeps R support Df Da)).
+          { rewrite mem_reduceDeps.
+            right; right; right; left; exists pn, pv, f, n, vs.
+            split; [exact Hda | split; [reflexivity | split; reflexivity]]. }
+          destruct (Hdep _ Hf _ _ Hd) as [v0 [Hv0 Hv0S]].
+          rewrite mem_embedVS in Hv0.
+          exists v0; split; [exact Hv0 |].
+          exists (featsOf n v0 S); split.
+          * intros x Hx; exfalso; exact (FSet.empty_spec Hx).
+          * apply mem_featureResolution; exists n, v0;
+              split; [exact Hv0S | reflexivity].
+        + destruct (FSet.choose_nonempty _ E) as [f0 Hf0].
+          assert (Hd0 : T.DepRel.In
+                          ((Name.FeatPkg pn f, pv),
+                           (Name.FeatPkg n f0, embedVS vs))
+                          (reduceDeps R support Df Da)).
+          { rewrite mem_reduceDeps.
+            right; right; right; right; exists pn, pv, f, n, vs, fs, f0.
+            split; [exact Hda | split; [exact E | split; [exact Hf0 |]]].
+            split; [reflexivity | split; reflexivity]. }
+          destruct (Hdep _ Hf _ _ Hd0) as [v0 [Hv0 Hv0S]].
+          rewrite mem_embedVS in Hv0.
+          pose proof (HfeatOrig _ _ _ Hv0S) as HvO.
+          exists v0; split; [exact Hv0 |].
+          exists (featsOf n v0 S); split.
+          * intros f' Hf'; rewrite featsOf_spec.
+            assert (Hd' : T.DepRel.In
+                            ((Name.FeatPkg pn f, pv),
+                             (Name.FeatPkg n f', embedVS vs))
+                            (reduceDeps R support Df Da)).
+            { rewrite mem_reduceDeps.
+              right; right; right; right; exists pn, pv, f, n, vs, fs, f'.
+              split; [exact Hda | split; [exact E | split; [exact Hf' |]]].
+              split; [reflexivity | split; reflexivity]. }
+            destruct (Hdep _ Hf _ _ Hd') as [v' [Hv' Hv'S]].
+            pose proof (HfeatOrig _ _ _ Hv'S) as Hv'O.
+            assert (Ev : v0 = v') by exact (Huniq (Name.Orig n) v0 v' HvO Hv'O).
+            rewrite Ev; exact Hv'S.
+          * apply mem_featureResolution; exists n, v0;
+              split; [exact HvO | reflexivity].
+      - intros n v v' fs fs' H1 H2.
+        apply mem_featureResolution in H1; destruct H1 as [n1 [v1 [HS1 Heq1]]].
+        apply mem_featureResolution in H2; destruct H2 as [n2 [v2 [HS2 Heq2]]].
+        injection Heq1 as E1 E2 E3; subst n1 v1 fs.
+        injection Heq2 as E4 E5 E6; subst n2 v2 fs'.
+        assert (Ev : v = v') by exact (Huniq (Name.Orig n) v v' HS1 HS2).
+        rewrite Ev; reflexivity.
+      - intros n v v' fs fs' H1 H2.
+        apply mem_featureResolution in H1; destruct H1 as [n1 [v1 [HS1 Heq1]]].
+        apply mem_featureResolution in H2; destruct H2 as [n2 [v2 [HS2 Heq2]]].
+        injection Heq1 as E1 E2 E3; subst n1 v1 fs.
+        injection Heq2 as E4 E5 E6; subst n2 v2 fs'.
+        exact (Huniq (Name.Orig n) v v' HS1 HS2).
+      - intros n v fs f Hmem Hf.
+        apply mem_featureResolution in Hmem;
+          destruct Hmem as [n1 [v1 [HS Heq]]].
+        injection Heq as E1 E2 E3; subst n1 v1 fs.
+        rewrite featsOf_spec in Hf.
+        pose proof (Hsub _ Hf) as HF; rewrite mem_reduceReal in HF.
+        destruct HF as [[p [HpR Hq]] | [n' [v' [f' [Hsupp [HR Hq]]]]]].
+        + destruct p as [pn pv]; unfold embedPkg in Hq; simpl in Hq;
+            discriminate Hq.
+        + injection Hq as E4 E5 E6; subst n' f' v'.
+          exact Hsupp.
+    Qed.
+
+    Module SOsw := SetOps Featured T.Pkg FeaturedSet T.PkgSet.
+    Module SOft := SetOps F T.Pkg FSet T.PkgSet.
+    Definition coreResolution (S_f : FeaturedSet.t) : T.PkgSet.t :=
+      T.PkgSet.union
+        (SOsw.map (fun '((n, v), _) => (Name.Orig n, v)) S_f)
+        (SOsw.unionMap (fun '((n, v), fs) =>
+             SOft.map (fun f => (Name.FeatPkg n f, v)) fs)
+           S_f).
+
+    Lemma mem_coreResolution : forall S_f (q : T.Pkg.t),
+        T.PkgSet.In q (coreResolution S_f) <->
+        (exists n v fs,
+           FeaturedSet.In ((n, v), fs) S_f /\ q = (Name.Orig n, v)) \/
+        (exists n v fs f, FeaturedSet.In ((n, v), fs) S_f /\ FSet.In f fs /\
+           q = (Name.FeatPkg n f, v)).
+    Proof.
+      intros S_f q; unfold coreResolution.
+      rewrite T.PkgSet.union_spec, SOsw.mem_map, SOsw.mem_unionMap.
+      split.
+      - intros [[[[pn pv] fs0] [HxS Hy]] | [[[pn pv] fs0] [HxS Hy]]];
+          cbn beta iota in Hy.
+        + left; exists pn, pv, fs0; split; [exact HxS | exact Hy].
+        + apply SOft.mem_map in Hy; destruct Hy as [f [Hf Hy]].
+          right; exists pn, pv, fs0, f;
+            split; [exact HxS | split; [exact Hf | exact Hy]].
+      - intros [[n [v [fs [HxS ->]]]] | [n [v [fs [f [HxS [Hf ->]]]]]]].
+        + left; exists ((n, v), fs); split; [exact HxS | reflexivity].
+        + right; exists ((n, v), fs); split; [exact HxS | cbn beta iota].
+          apply SOft.mem_map; exists f; split; [exact Hf | reflexivity].
+    Qed.
+
+    Theorem feature_completeness :
+      forall (R : PkgSet.t) (support : SupportSet.t)
+             (Df : FeatDepRel.t) (Da : AddlDepRel.t)
+             (r : Pkg.t) (S_f : FeaturedSet.t),
+        IsResolution R support Df Da r S_f ->
+        T.IsResolution (reduceReal R support) (reduceDeps R support Df Da)
+          (embedPkg r) (coreResolution S_f).
+    Proof.
+      intros R support Df Da r S_f Hres.
+      destruct Hres as [Hnrs Hsubset Hrootm Hdepc Haddlc Hfu Hvu Hsm].
+      destruct r as [rn rv].
+      constructor.
+      - intros q Hq.
+        rewrite mem_coreResolution in Hq.
+        rewrite mem_reduceReal.
+        destruct Hq as [[n [v [fs [HS ->]]]] | [n [v [fs [f [HS [Hf ->]]]]]]].
+        + left; exists (n, v); split; [exact (Hsubset _ _ HS) | reflexivity].
+        + right; exists n, v, f.
+          split; [exact (Hsm n v fs f HS Hf) |].
+          split; [exact (Hsubset _ _ HS) | reflexivity].
+      - rewrite mem_coreResolution.
+        left; exists rn, rv, FSet.empty; split; [exact Hrootm | reflexivity].
+      - intros q Hq m vs Hd.
+        rewrite mem_coreResolution in Hq.
+        rewrite mem_reduceDeps in Hd.
+        destruct Hq as [[pn [pv [fs [HS Hq]]]] |
+                        [pn [pv [fs [f0 [HS [Hf0 Hq]]]]]]]; subst q.
+        + destruct Hd as [D1 | [D2 | [D3 | [D4 | D5]]]].
+          * destruct D1 as [n [v [f [_ [_ [Hsrc _]]]]]]; discriminate Hsrc.
+          * destruct D2 as [q' [m' [vs' [Hdf [Hsrc [Htn Htvs]]]]]]; subst m vs.
+            destruct q' as [qn qv]; unfold embedPkg in Hsrc; simpl in Hsrc.
+            injection Hsrc as E1 E2; subst qn qv.
+            destruct (Hdepc _ _ HS _ _ _ Hdf) as [v' [Hv' [fs' [_ Hfs']]]].
+            exists v'; split; [rewrite mem_embedVS; exact Hv' |].
+            rewrite mem_coreResolution.
+            left; exists m', v', fs'; split; [exact Hfs' | reflexivity].
+          * destruct D3
+              as [q' [m' [vs' [fs0 [f [Hdf [E0 [Hf [Hsrc [Htn Htvs]]]]]]]]]];
+              subst m vs.
+            destruct q' as [qn qv]; unfold embedPkg in Hsrc; simpl in Hsrc.
+            injection Hsrc as E1 E2; subst qn qv.
+            destruct (Hdepc _ _ HS _ _ _ Hdf) as [v' [Hv' [fs' [Hsub' Hfs']]]].
+            exists v'; split; [rewrite mem_embedVS; exact Hv' |].
+            rewrite mem_coreResolution.
+            right; exists m', v', fs', f.
+            split; [exact Hfs' | split; [exact (Hsub' _ Hf) | reflexivity]].
+          * destruct D4 as [n [v [f [m' [vs' [_ [Hsrc _]]]]]]];
+              discriminate Hsrc.
+          * destruct D5 as
+              [n [v [f [m' [vs' [fs0 [f' [_ [_ [_ [Hsrc _]]]]]]]]]]];
+              discriminate Hsrc.
+        + destruct Hd as [D1 | [D2 | [D3 | [D4 | D5]]]].
+          * destruct D1 as [n [v [f [Hsupp [HR [Hsrc [Htn Htvs]]]]]]];
+              subst m vs.
+            injection Hsrc as E1 E2 E3; subst n f v.
+            exists pv; split; [rewrite SOvt.singleton_in; reflexivity |].
+            rewrite mem_coreResolution.
+            left; exists pn, pv, fs; split; [exact HS | reflexivity].
+          * destruct D2 as [q' [m' [vs' [_ [Hsrc _]]]]].
+            destruct q' as [qn qv]; unfold embedPkg in Hsrc; simpl in Hsrc;
+              discriminate Hsrc.
+          * destruct D3 as [q' [m' [vs' [fs0 [f [_ [_ [_ [Hsrc _]]]]]]]]].
+            destruct q' as [qn qv]; unfold embedPkg in Hsrc; simpl in Hsrc;
+              discriminate Hsrc.
+          * destruct D4 as [n [v [f [m' [vs' [Hda [Hsrc [Htn Htvs]]]]]]]];
+              subst m vs.
+            injection Hsrc as E1 E2 E3; subst n f v.
+            destruct (Haddlc _ _ HS f0 Hf0 _ _ _ Hda)
+              as [v' [Hv' [fs' [_ Hfs']]]].
+            exists v'; split; [rewrite mem_embedVS; exact Hv' |].
+            rewrite mem_coreResolution.
+            left; exists m', v', fs'; split; [exact Hfs' | reflexivity].
+          * destruct D5 as [n [v [f [m' [vs' [fs0 [f'
+                            [Hda [E0 [Hf' [Hsrc [Htn Htvs]]]]]]]]]]]];
+              subst m vs.
+            injection Hsrc as E1 E2 E3; subst n f v.
+            destruct (Haddlc _ _ HS f0 Hf0 _ _ _ Hda)
+              as [v' [Hv' [fs' [Hsub' Hfs']]]].
+            exists v'; split; [rewrite mem_embedVS; exact Hv' |].
+            rewrite mem_coreResolution.
+            right; exists m', v', fs', f'.
+            split; [exact Hfs' | split; [exact (Hsub' _ Hf') | reflexivity]].
+      - intros nm v1 v2 H1 H2.
+        rewrite mem_coreResolution in H1, H2.
+        destruct H1 as [[n1 [w1 [fs1 [HS1 Hq1]]]] |
+                        [n1 [w1 [fs1 [f1 [HS1 [Hf1 Hq1]]]]]]];
+          destruct H2 as [[n2 [w2 [fs2 [HS2 Hq2]]]] |
+                          [n2 [w2 [fs2 [f2 [HS2 [Hf2 Hq2]]]]]]].
+        + injection Hq1 as E1 E2; subst nm v1.
+          injection Hq2 as E3 E4; subst n2 v2.
+          exact (Hvu _ _ _ _ _ HS1 HS2).
+        + injection Hq1 as E1 E2; subst nm v1.
+          discriminate Hq2.
+        + injection Hq1 as E1 E2; subst nm v1.
+          discriminate Hq2.
+        + injection Hq1 as E1 E2; subst nm v1.
+          injection Hq2 as E3 E4 E5; subst n2 f2 v2.
+          exact (Hvu _ _ _ _ _ HS1 HS2).
+    Qed.
+  End Reduction.
+
+End Feature.
